% !TeX root = Asparsi.tex
% !BIB TS-program = biber
% !TeX encoding = UTF-8
% !TeX spellcheck = it_IT
\chapter{Scomposizioni}\label{ch:scomposizioni}
\section{Scomposizioni di polinomi}
\begin{thm}[Scomposizioni di polinomi]\label{thm:scomposizioni}
\begin{align}
(a+b)^2=&{}a^2+b^2+2ab\\
(a-b)^2=&{}a^2+b^2-2ab\\
a^2-b^2=&{}(a-b)(a+b)\\
a^2+b^2=&{}(a+b)^2-2ab\\
a^2+b^2=&{}(a-b)^2+2ab\\
a^3+b^3=&{}(a+b)[(a+b)^2-3ab]\label{eq:ascomp1}\\
a^3-b^3=&{}(a-(b)[(a-b)^2+3ab]\label{eq:ascomp2}\\
a^3+b^3=&{}(a+b)(a^2-ab+b^2)\label{eq:ascomp3}\\
a^3-b^3=&{}(a-b)(a^2+ab+b^2)\label{eq:ascomp4}\\
2(a^2+b^2)=&{}(a+b)^2+(a-b)^2\label{eq:ascomp5}\\
4ab=&{}(a+b)^2-(a-b)^2\label{eq:ascomp6}\\
a^4-b^4=&{}(a-b)(a+b)[(a+b)^2-2ab]\label{eq:ascomp7}\\
(a-b)^2=&{}(a+b)^2-4ab\label{eq:ascomp8}\\
(a+b)^2=&{}(a-b)^2+4ab\label{eq:ascomp9}\\
a^4+b^4=&{}[(a+b)^2-2ab]^2-2(ab)^2\label{eq:ascomp10}\\
(a+b+c)^3=&{}a^3 + 3a^2b + 3a^2c + 3ab^2 + 6abc + 3ac^2 + b^3 + 3b^2c + 3bc^2 + c^3\\
a^3+b^3+c^3-3abc=&{}(a+b+c)(a^2+b^2+c^2-ab-bc-ac)\label{eq:ascomp11}\\
a^4+a^2+1=&{}(a^2+a+1)(a^2-a+1)\label{eq:ascomp12}\\
a^2+b^2+c^2=&{}(a+b+c)^2-2(ab+ac+bc)\label{eq:ascomp13}\\
\end{align}
segue
\end{thm}
\begin{proof}
	Dimostriamo \ref{eq:ascomp1}
	\begin{align*}
	a^3+b^3=&{}(a+b)^3-3a^2b-3ab^2\\
	=&{}(a+b)^3-3ab(a+b)\\
	=&{}(a+b)[(a+b)^2-3ab]\\
	\end{align*}
	cvd
	
		Dimostriamo \ref{eq:ascomp2}
	\begin{align*}
	a^3-b^3=&{}(a-b)^3+3a^2b-3ab^2\\
	=&{}(a-b)^3+3ab(a-b)\\
	=&{}(a-b)[(a-b)^2+3ab]\\
	\end{align*}
	cvd
	
		Dimostriamo \ref{eq:ascomp3}
	\begin{align*}
	a^3+b^3=&{}(a+b)^3-3a^2b-3ab^2\\
	=&{}(a+b)^3-3ab(a+b)\\
	=&{}(a+b)[(a+b)^2-3ab]\\
	=&{}(a+b)[a^2+b^2+2ab-3ab]\\
	=&{}(a+b)(a^2-ab+b^2)\\
	\end{align*}
	cvd
	
	Dimostriamo \ref{eq:ascomp4}
	\begin{align*}
	a^3-b^3=&{}(a-b)^3+3a^2b-3ab^2\\
	=&{}(a-b)^3+3ab(a-b)\\
	=&{}(a-b)[(a-b)^2+3ab]\\
	=&{}(a-b)[a^2+b^2-2ab+3ab]\\
	=&{}(a-b)(a^2+ab+b^2)\\
	\end{align*}
	cvd
	
		Dimostriamo \ref{eq:ascomp5}
	\begin{align*}
(a+b)^2+(a-b)^2=&a^2+b^2+2ab+a^2+b^2-2ab\\
=&2(a^2+b^2)\\
	\end{align*}
	cvd
	
		Dimostriamo \ref{eq:ascomp6}
\begin{align*}
(a+b)^2-(a-b)^2=&a^2+b^2+2ab-a^2-b^2+2ab\\
=&4ab\\
\end{align*}
cvd

		Dimostriamo \ref{eq:ascomp7}
\begin{align*}
a^4-b^4=&{}(a^2-b^2)(a^2+b^2)\\
=&{}(a-b)(a+b)[(a+b)^2-2ab]\\
\end{align*}
cvd

Dimostriamo \ref{eq:ascomp8}
\begin{align*}
(a-b)^2=&a^2+b^2-2ab\\
=&a^2+b^2+2ab-2ab-2ab\\
=&{}(a+b)^2-4ab
\end{align*}
cvd

Dimostriamo \ref{eq:ascomp9}
\begin{align*}
(a+b)^2=&a^2+b^2+2ab\\
=&a^2+b^2-2ab+2ab+2ab\\
=&{}(a-b)^2+4ab
\end{align*}
cvd

Dimostriamo \ref{eq:ascomp10}
\begin{align*}
a^4+b^4=&{}(a+b)^4-4a^3b-4ab^3-6a^2b^2\\
=&{}(a+b)^4+4a^2b^2-4a^3b-4ab^3-8a^2b^2-2a^2b^2\\
=&{}(a+b)^4+4a^2b^2-4ab(a^2+b^2+2ab)-2a^2b^2\\
=&{}(a+b)^4+4a^2b^2-4ab(a+b)^2-2a^2b^2\\
=&{}[(a+b)^2-2ab]^2-2(ab)^2
\end{align*}

cvd

Dimostriamo \ref{eq:ascomp11}
\begin{align*}
a^3+b^3+c^3=&\\
=&a^3+b^3+c^3+\\
+&ab^2-ab^2+ac^2-ac^2+\\
+&a^2b-a^2b+bc^2-bc^2+\\
+&a^2c-a^2c+b^2c-b^2c+\\
-&abc-abc-abc+3abc\\
=&a^3+a^2b+a^2c+\\
+&b^3+ab^2+b^2c+\\
+&c^3+ac^2+bc^2+\\
-&ab^2-a^2c-abc+\\
-&bc^2-b^2c-abc+\\
-&ac^2-a^2c-abc\\
+&abc\\
=&a^2(a+b+c)+\\
+&b^2(b+a+c)+\\
+&c^2(c+a+b)+\\
-&ab(b+a+c)+\\
-&bc(c+b+a)+\\
-&ac(c+a+b)+\\
+&3abc\\
=&{}(a+b+c)(a^2+b^2+c^2-ab-bc-ac)+3abc\\
\end{align*}
cvd

Dimostriamo \ref{eq:ascomp12}
\begin{align*}
a^4+a^2+1=&\\
=&a^4-a^3+a^2+a^3-a^2+a+a^2-a+1\\
=&a^4-a^3+a^2\\
+&a^3-a^2+a+\\
+&a^2-a+1\\
=a^2(a^2+a+1)-a(a^2+a+1)+1(a^2+a+1)\\
=(a^2+a+1)(a^2-a+1)
\end{align*}
cvd
\end{proof}